# RLC Analytical Responses 

John Morrow

Equation 1 is the differential equation for the series-connected RLC circuit (Figure 1 ) in terms of $i$, the current flowing in the circuit. $R, L$, and $C$ represent the resistance, inductance, and capacitance.

$$
\begin{equation*}
L \frac{d i^{2}}{d t^{2}}+R \frac{d i}{d t}+\frac{1}{C}=0 \tag{1}
\end{equation*}
$$



Figure 1: Series-connected RLC circuit

Taking the Laplace transform of each term in Equation 1:

$$
\begin{align*}
\mathcal{L}\left\{L \frac{d i^{2}}{d t^{2}}\right\} & =L\left(s^{2} F(s)-s i(0)-i^{\prime}(0)\right)  \tag{2}\\
\mathcal{L}\left\{R \frac{d i}{d t}\right\} & =R(s F(s)-i(0))  \tag{3}\\
\mathcal{L}\left\{\frac{1}{C} i\right\} & =\frac{1}{C} F(s) \tag{4}
\end{align*}
$$

Combining and collecting terms, the Laplace transform of Equation 1 is:

$$
\begin{equation*}
\left(L s^{2}+R s+\frac{1}{C}\right) F(s)-(s+1) i(0)-i^{\prime}(0)=0 \tag{5}
\end{equation*}
$$

Solving for $F(s)$ :

$$
\begin{equation*}
F(s)=\frac{(s+1) i(0)+i^{\prime}(0)}{L s^{2}+R s+\frac{1}{C}} \tag{6}
\end{equation*}
$$

Applying the initial conditions, $i(0)=0$ and $i^{\prime}(0)=\frac{V(0)}{L}$
where $V(0)$ is the initial capacitor voltage at $t=0$ :

$$
\begin{equation*}
F(s)=\frac{\frac{V(0)}{L}}{L s^{2}+R s+\frac{1}{C}} \tag{7}
\end{equation*}
$$

Factoring the denominator of Equation 7 and substituting $\alpha=\frac{R}{2 L}$ :

$$
\begin{equation*}
\left(s+\alpha+\sqrt{\alpha^{2}-\frac{1}{L C}}\right)\left(s+\alpha-\sqrt{\alpha^{2}-\frac{1}{L C}}\right) \tag{8}
\end{equation*}
$$

Simplifying further by substituting $z=\sqrt{\alpha^{2}-\frac{1}{L C}}$, the roots of $F(s)$ are:

$$
\begin{equation*}
(s+\alpha-z)(s+\alpha+z) \tag{9}
\end{equation*}
$$

## under-damped response

For the under-damped case, where $\alpha<\sqrt{\frac{1}{L C}}, z$ becomes imaginary (denoted here by $j$ ):

$$
\begin{equation*}
(s+\alpha-z j)(s+\alpha+z j) \tag{18}
\end{equation*}
$$

Expressing $F(s)$ from Equation 7 with partial fractions:

$$
\begin{align*}
& F(s)=\left(\frac{\frac{V(0)}{L}}{(s+\alpha-z j)(s+\alpha+z j)}\right)=\frac{A}{s+\alpha+z j}+\frac{B}{s+\alpha-z j}  \tag{11}\\
& F(s)=\frac{\frac{V(0)}{L}}{(s+\alpha-z j)(s+\alpha+z j)}=\frac{A(s+\alpha-z j)+B(s+\alpha+z j)}{(s+\alpha-z j)(s+\alpha+z j)} \tag{12}
\end{align*}
$$

Equating the numerators in Equation 12:

$$
\begin{equation*}
\frac{V(0)}{L}=A(s+\alpha-z j)+B(s+\alpha+z j) \tag{13}
\end{equation*}
$$

When $s=-\alpha-z j$, Equation 13 becomes:

$$
\begin{equation*}
\frac{V(0)}{L}=A(-2 z j) \tag{14}
\end{equation*}
$$

Solving for $A$ :

$$
\begin{equation*}
A=\frac{V(0)}{(-2 z j) L}\left(\frac{j}{j}\right)=\frac{V(0) j}{2 z L} \tag{15}
\end{equation*}
$$

When $s=-\alpha+z j$, Equation 13 becomes:

$$
\begin{equation*}
\frac{V(0)}{L}=B(2 z j) \tag{16}
\end{equation*}
$$

Solving for $B$ :

$$
\begin{equation*}
B=\frac{V(0)}{(2 z j) L}\left(\frac{j}{j}\right)=\frac{-V(0) j}{2 z L} \tag{17}
\end{equation*}
$$

Substituting these values for $A$ and $B$ into Equation 11:

$$
\begin{equation*}
F(s)=\frac{\frac{V(0) j}{2 z L}}{s+\alpha+z j}+\frac{\frac{-V(0) j}{2 z L}}{s+\alpha-z j} \tag{18}
\end{equation*}
$$

Taking the inverse Laplace transform of $F(s)$ :

$$
\begin{align*}
i(t) & =\mathcal{L}^{-1} F(s)  \tag{19}\\
i(t) & =\frac{V(0)}{2 z L}\left(j e^{-(\alpha+z j) t}-j e^{-(\alpha-z j) t}\right)  \tag{20}\\
i(t) & =\frac{V(0)}{2 z L} e^{-\alpha t} j\left(\frac{j}{j}\right)\left(e^{-z j t}-e^{z j t}\right)  \tag{21}\\
i(t) & =\frac{V(0)}{z L} e^{-\alpha t} \frac{\left(e^{z j t}-e^{-z j t}\right)}{2 j} \tag{22}
\end{align*}
$$

Substituting the identity $\sin (x)=\frac{\left(e^{j x}-e^{-j x}\right)}{2 j}$ :

$$
\begin{equation*}
i(t)=\frac{V(0)}{z L} e^{-\alpha t} \sin (z t) \tag{23}
\end{equation*}
$$

Figure 2 is the response of Equation 23, with $R=1.2$ (ohms), $L=1.5$ (henries), $C=0.3$ (farads), and $V(0)=12$ (volts). With these component values, $\alpha=0.4$ and $z=1.44$.


Figure 2: Under-damped response

## critically-damped response

For the critically-damped case, $\alpha=\sqrt{\frac{1}{L C}}$. This results in $z=0$, and both roots of $F(s)$ in Equation 9 are identical.

$$
\begin{equation*}
(s+\alpha)(s+\alpha) \tag{24}
\end{equation*}
$$

Expressing $\mathrm{F}(\mathrm{s})$ from Equation 7 with partial fractions and two identical roots:

$$
\begin{align*}
& F(s)=\left(\frac{\frac{V(0)}{L}}{(s+\alpha)(s+\alpha)}\right)=\frac{A}{s+\alpha}+\frac{B}{(s+\alpha)^{2}}  \tag{25}\\
& F(s)=\frac{\frac{V(0)}{L}}{(s+\alpha)(s+\alpha)}=\frac{A(s+\alpha)+B}{(s+\alpha)^{2}} \tag{26}
\end{align*}
$$

Equating the numerators in Equation 26:

$$
\begin{equation*}
\frac{V(0)}{L}=A(s+\alpha)+B \tag{27}
\end{equation*}
$$

When $s=-\alpha$, Equation 27 becomes:

$$
\begin{equation*}
\frac{V(0)}{L}=A(-\alpha+\alpha)+B \tag{28}
\end{equation*}
$$

Solving for $B$ and $A$ :

$$
\begin{equation*}
B=\frac{V(0)}{L}, \quad A=0 \tag{29}
\end{equation*}
$$

Substituting the values for $A$ and $B$ into Equation 25:

$$
\begin{equation*}
F(s)=\frac{\frac{V(0)}{L}}{(s+\alpha)^{2}} \tag{30}
\end{equation*}
$$

Taking the inverse Laplace transform of $F(s)$ :

$$
\begin{align*}
& i(t)=\mathcal{L}^{-1} F(s)  \tag{31}\\
& i(t)=\frac{V(0)}{L} t e^{-\alpha t} \tag{32}
\end{align*}
$$

Figure 3 is the response of Equation 32, with $R=4.47$ (ohms), $L=1.5$ (henries), $C=0.3$ (farads), and $V(0)=12$ (volts). With these component values, $\alpha=1.49$.


Figure 3: Critically-damped response

## over-damped response

For the over-damped case, $\alpha>\sqrt{\frac{1}{L C}}$. Expressing $F(s)$ from Equation 7 with partial fractions:

$$
\begin{align*}
& F(s)=\left(\frac{\frac{V(0)}{L}}{(s+\alpha-z)(s+\alpha+z)}\right)=\frac{A}{s+\alpha+z}+\frac{B}{s+\alpha-z}  \tag{33}\\
& F(s)=\frac{\frac{V(0)}{L}}{(s+\alpha-z j)(s+\alpha+z j)}=\frac{A(s+\alpha-z)+B(s+\alpha+z)}{(s+\alpha-z)(s+\alpha+z)} \tag{34}
\end{align*}
$$

Equating the numerators in Equation 34:

$$
\begin{equation*}
\frac{V(0)}{L}=A(s+\alpha-z)+B(s+\alpha+z) \tag{35}
\end{equation*}
$$

When $s=-\alpha-z$, Equation 35 becomes:

$$
\begin{equation*}
\frac{V(0)}{L}=A(-2 z) \tag{36}
\end{equation*}
$$

Solving for $A$ :

$$
\begin{equation*}
A=\frac{V(0)}{-2 z L} \tag{37}
\end{equation*}
$$

When $s=-\alpha+z$, Equation 35 becomes:

$$
\begin{equation*}
\frac{V(0)}{L}=B(2 z) \tag{38}
\end{equation*}
$$

Solving for $B$ :

$$
\begin{equation*}
B=\frac{V(0)}{2 z L} \tag{39}
\end{equation*}
$$

Substituting the values for $A$ and $B$ into Equation 33:

$$
\begin{equation*}
F(s)=\frac{V(0)}{2 z L}\left(\frac{1}{s+\alpha-z}-\frac{1}{s+\alpha+z}\right) \tag{4Q}
\end{equation*}
$$

Taking the inverse Laplace transform of $F(s)$ :

$$
\begin{align*}
& i(t)=\mathcal{L}^{-1} F(s)  \tag{41}\\
& i(t)=\frac{V(0)}{2 z L}\left(e^{(-\alpha+z) t}-e^{(-\alpha-z) t}\right) \tag{42}
\end{align*}
$$

Figure 4 is the response of Equation 42, with $R=6.0$ (ohms), $L=1.5$ (henries), $C=0.3$ (farads), and $V(0)=12$ (volts). With these component values, $\alpha=2.0$ and $z=1.33$.


Figure 4: Over-damped response

